Vizing/new/Fan.lean
@@ -21,22 +21,22 @@ a maximal fan from an edge (x, y).
 
 -/
 
-variable (n : Nat) (c : Nat) (G : Graph n) (C : EdgeColoring n c G)
+variable {n : Nat} {c : Nat} (G : Graph n) (C : EdgeColoring c G)
 
 def colorAx (F : Array (Vertex n)) (x : Vertex n) :=
   ∀ i, (h : i < (F.size - 1)) →
-  (color n c G C (x, F[i + 1]'(by exact Nat.add_lt_of_lt_sub h))) ∈
-  (freeColorsOn n c G C F[i])
+  (color c G C (x, F[i + 1]'(by exact Nat.add_lt_of_lt_sub h))) ∈
+  (freeColorsOn G C F[i])
 
 structure Fan (x y : Vertex n) where
   val : Array (Vertex n)
-  nborsAx : val.toList ⊆ (nbhd n G x).val
+  nborsAx : val.toList ⊆ (nbhd G x).val
   nonemptyAx : val ≠ #[]
   firstElemAx : val[0]'(by exact Array.size_pos_iff.mpr nonemptyAx) = y
-  colorAx : colorAx n c G C val x
+  colorAx : colorAx G C val x
   nodupAx : val.toList.Nodup
 
-def default (x y : Vertex n) (h : present n G (x, y)) : Fan n c G C x y where
+def default (x y : Vertex n) (h : present G (x, y)) : Fan G C x y where
   val := #[y]
   nborsAx := by
     simp
@@ -49,7 +49,7 @@ def default (x y : Vertex n) (h : present n G (x, y)) : Fan n c G C x y where
 def add (x y : Vertex n) (F : Array (Vertex n)) (nbors : List (Vertex n))
   (h : F ≠ #[]) :=
   match (List.attach nbors).find? (fun ⟨z, _⟩ ↦
-    color n c G C (x, z) ∈ freeColorsOn n c G C (F.back (Array.size_pos_iff.mpr h))) with
+    color c G C (x, z) ∈ freeColorsOn G C (F.back (Array.size_pos_iff.mpr h))) with
   | some z => add x y (F.push z.val) (nbors.erase z.val) Array.push_ne_empty
   | none => F
   termination_by nbors.length
@@ -61,32 +61,41 @@ def add (x y : Vertex n) (F : Array (Vertex n)) (nbors : List (Vertex n))
     rfl
 
 theorem add_nborsAx (x y : Vertex n) (F : Array (Vertex n))
-  (nbors : List (Vertex n)) (hne : F ≠ #[]) (h : F.toList ⊆ nbhd n G x)
-  (hn : nbors ⊆ nbhd n G x) :
-  (add n c G C x y F nbors hne).toList ⊆ nbhd n G x := by
-  induction F, nbors, hne using add.induct n c G C x
+  (nbors : List (Vertex n)) (hne : F ≠ #[]) (h : F.toList ⊆ (nbhd G x).val)
+  (hn : nbors ⊆ (nbhd G x).val) :
+  (add G C x y F nbors hne).toList ⊆ (nbhd G x).val := by
+  fun_induction add G C x y F nbors hne
   · rename_i F nbors hne z hz ih
-    rw [add]; simp_all
+    simp_all
     apply ih
     · exact hn z.prop
     · grw [List.erase_subset]; assumption
-  · rename_i nbors _ _ hz
-    rw [add, hz]; simp_all
+  · simp_all
 
 theorem add_nonemptyAx (x y : Vertex n) (F : Array (Vertex n))
   (nbors : List (Vertex n)) (hne : F ≠ #[]) :
-  (add n c G C x y F nbors hne) ≠ #[] := by
-  induction F, nbors, hne using add.induct n c G C x
-  · rw [add]; simp_all
-  · rename_i hz
-    rw [add, hz]; simp_all
+  (add G C x y F nbors hne) ≠ #[] := by
+  fun_induction add G C x y F nbors hne <;> simp_all
+
+theorem add_maximal (x y : Vertex n) (F : Array (Vertex n))
+  (nbors : List (Vertex n)) (hne : F ≠ #[]) :
+  ∀ z ∈ nbors, z ∉ (add G C x y F nbors hne) →
+    color c G C (x, z) ∉ (freeColorsOn G C
+    ((add G C x y F nbors hne).back (Array.size_pos_iff.mpr
+      (add_nonemptyAx G C x y F nbors hne)))) := by
+  fun_cases add G C x y F nbors hne
+  unfold add
+  simp_all
+
+  stop
+  sorry
 
 theorem add_firstElemAx (x y : Vertex n) (F : Array (Vertex n))
   (nbors : List (Vertex n)) (hne : F ≠ #[])
   (h : F[0]'(Array.size_pos_iff.mpr hne) = y) :
-  (add n c G C x y F nbors hne)[0]'(Array.size_pos_iff.mpr
-    (add_nonemptyAx n c G C x y F nbors hne)) = y := by
-  induction F, nbors, hne using add.induct n c G C x
+  (add G C x y F nbors hne)[0]'(Array.size_pos_iff.mpr
+    (add_nonemptyAx G C x y F nbors hne)) = y := by
+  fun_induction add G C x y F nbors hne
   · rename_i F nbors hne z hz ih
     unfold add; simp_all only
     apply ih
@@ -94,12 +103,12 @@ theorem add_firstElemAx (x y : Vertex n) (F : Array (Vertex n))
   · unfold add; simp_all only
 
 theorem add_colorAx (x y : Vertex n) (F : Array (Vertex n))
-  (nbors : List (Vertex n)) (hne : F ≠ #[]) (h : colorAx n c G C F x) :
-  colorAx n c G C (add n c G C x y F nbors hne) x := by
+  (nbors : List (Vertex n)) (hne : F ≠ #[]) (h : colorAx G C F x) :
+  colorAx G C (add G C x y F nbors hne) x := by
   simp [colorAx]
-  induction F, nbors, hne using add.induct n c G C x
+  fun_induction add G C x y F nbors hne
   · rename_i F nbors hne z hz ih
-    rw [add]; simp_all only
+    simp_all only
     apply ih
     simp [colorAx] at ⊢ h
     intro i hi
@@ -114,16 +123,15 @@ theorem add_colorAx (x y : Vertex n) (F : Array (Vertex n))
       simp [Nat.sub_add_cancel (Nat.one_le_of_lt hi), Array.getElem_push_lt hi]
       apply List.find?_some at hz; simp [Array.back] at hz
       exact hz
-  · rw [add]
-    simp_all only [colorAx, implies_true]
+  · simp_all only [colorAx, implies_true]
 
 theorem add_nodupAx (x y : Vertex n) (F : Array (Vertex n))
   (nbors : List (Vertex n)) (hn : nbors.Nodup) (hne : F ≠ #[]) (h : F.toList.Nodup)
   (hdisjoint : List.Disjoint nbors F.toList) :
-  (add n c G C x y F nbors hne).toList.Nodup := by
-  induction F, nbors, hne using add.induct n c G C x
+  (add G C x y F nbors hne).toList.Nodup := by
+  fun_induction add G C x y F nbors hne
   · rename_i F nbors hne z hz ih
-    rw [add]; simp_all only
+    simp_all only
     apply ih
     · exact List.Nodup.erase z.val hn
     · simp
@@ -139,17 +147,16 @@ theorem add_nodupAx (x y : Vertex n) (F : Array (Vertex n))
       · by_contra ha
         subst ha
         exact List.Nodup.not_mem_erase hn h
-  · rw [add]; simp_all only
+  · simp_all only
 
-
-def mkMaxFan (x y : Vertex n) (h : present n G (x, y)) : Array (Vertex n) :=
-  add n c G C x y (default n c G C x y h).val
-  ((nbhd n G x).val.erase y) (default n c G C x y h).nonemptyAx
+def mkMaxFan (x y : Vertex n) (h : present G (x, y)) : Array (Vertex n) :=
+  add G C x y (default G C x y h).val
+  ((nbhd G x).val.erase y) (default G C x y h).nonemptyAx
 
 variable (x y : Vertex n)
 
-theorem mkMaxFan_nborsAx (hpres : present n G (x, y)) :
-  (mkMaxFan n c G C x y hpres).toList ⊆ (nbhd n G x).val := by
+theorem mkMaxFan_nborsAx (hpres : present G (x, y)) :
+  (mkMaxFan G C x y hpres).toList ⊆ (nbhd G x).val := by
   simp [mkMaxFan, default]
   simp [present] at hpres
   apply add_nborsAx
@@ -157,37 +164,37 @@ theorem mkMaxFan_nborsAx (hpres : present n G (x, y)) :
     exact hpres.right
   · exact List.erase_subset
 
-theorem mkMaxFan_nonemptyAx (x y : Vertex n) (hpres : present n G (x, y)) :
-  mkMaxFan n c G C x y hpres ≠ #[] := by
+theorem mkMaxFan_nonemptyAx (x y : Vertex n) (hpres : present G (x, y)) :
+  mkMaxFan G C x y hpres ≠ #[] := by
   simp [mkMaxFan, default, add_nonemptyAx]
 
-theorem mkMaxFan_firstElemAx (x y : Vertex n) (hpres : present n G (x, y)) :
-  (mkMaxFan n c G C x y hpres)[0]'(by
-  exact Array.size_pos_iff.mpr (mkMaxFan_nonemptyAx n c G C x y hpres))
+theorem mkMaxFan_firstElemAx (x y : Vertex n) (hpres : present G (x, y)) :
+  (mkMaxFan G C x y hpres)[0]'(by
+  exact Array.size_pos_iff.mpr (mkMaxFan_nonemptyAx G C x y hpres))
   = y := by
   simp [mkMaxFan, default, add_firstElemAx]
 
-theorem mkMaxFan_colorAx (x y : Vertex n) (hpres : present n G (x, y)) :
-  colorAx n c G C (mkMaxFan n c G C x y hpres) x := by
-  simp [mkMaxFan, (default n c G C x y hpres).colorAx, add_colorAx]
+theorem mkMaxFan_colorAx (x y : Vertex n) (hpres : present G (x, y)) :
+  colorAx G C (mkMaxFan G C x y hpres) x := by
+  simp [mkMaxFan, (default G C x y hpres).colorAx, add_colorAx]
 
-theorem mkMaxFan_nodupAx (x y : Vertex n) (hpres : present n G (x, y)) :
-  (mkMaxFan n c G C x y hpres).toList.Nodup := by
+theorem mkMaxFan_nodupAx (x y : Vertex n) (hpres : present G (x, y)) :
+  (mkMaxFan G C x y hpres).toList.Nodup := by
   simp [mkMaxFan, default]
   apply add_nodupAx
   · apply List.Nodup.erase y
-    exact (nbhd n G x).prop.right
+    exact (nbhd G x).prop.right
   · exact List.nodup_singleton y
   · apply List.disjoint_singleton.mpr
     apply List.Nodup.not_mem_erase
-    exact (nbhd n G x).prop.right
+    exact (nbhd G x).prop.right
 
-def maximalFan (x y : Vertex n) (h : present n G (x, y)) : Fan n c G C x y where
-  val := mkMaxFan n c G C x y h
-  nborsAx := mkMaxFan_nborsAx n c G C x y h
-  firstElemAx := mkMaxFan_firstElemAx n c G C x y h
-  nonemptyAx := mkMaxFan_nonemptyAx n c G C x y h
-  colorAx := mkMaxFan_colorAx n c G C x y h
-  nodupAx := mkMaxFan_nodupAx n c G C x y h
+def maximalFan (x y : Vertex n) (h : present G (x, y)) : Fan G C x y where
+  val := mkMaxFan G C x y h
+  nborsAx := mkMaxFan_nborsAx G C x y h
+  firstElemAx := mkMaxFan_firstElemAx G C x y h
+  nonemptyAx := mkMaxFan_nonemptyAx G C x y h
+  colorAx := mkMaxFan_colorAx G C x y h
+  nodupAx := mkMaxFan_nodupAx G C x y h
 
 end Fan
