Vizing/new/Subfan.lean
@@ -12,13 +12,69 @@ open Fan
 
 /-
 
-A fan on (x, y) is a nonempty distinct list of vertices
-that are all adjacent to x such that
-the color of (x, F[i]) is free on F[i+1].
+Definition of a subfan:
 
-Definition/axioms for a fan, and implementation of a function that creates
-a maximal fan from an edge (x, y).
+H is a subfan of F if H is a fan such that H.val is a prefix of F.val.
+
+Proof that maximalFan is a maximal fan
 
 -/
+
+variable {n c : Nat} (G : Graph n) (C : EdgeColoring c G) (x y : Vertex n)
+  (h : present G (x, y))
+
+-- F1 is a subfan of F2
+def isSubfan (F1 F2 : Fan G C x y) :=
+  F1.val.isPrefixOf F2.val
+
+/-
+
+If F is a strict subfan of G, there exists an element we can add to F
+to create a larger fan.
+
+That is, there is a vertex z adjacent to x such that the color of (x, z) is free on F.back.
+
+Prefix -> equal or there exists another element we can add
+
+That element is adjacent to
+
+-/
+
+theorem maximalFan_spec : ∀ (F : Fan G C x y),
+  isSubfan G C x y (maximalFan G C x y h) F →
+  F.val = (maximalFan G C x y h).val := by
+  intro F hF
+  simp [isSubfan, ← Array.isPrefixOf_toList] at hF
+  rcases (lt_or_eq_of_le (List.IsPrefix.length_le hF)) with hlt | heq
+  · exfalso
+    have hsize := (Array.size_pos_iff.mpr (maximalFan G C x y h).nonemptyAx)
+    have ⟨_, aux0⟩ := List.prefix_iff_getElem.mp hF
+
+    apply List.prefix_iff_eq_append.mp at hF
+    rw [List.drop_eq_getElem_cons hlt] at hF
+
+    have := F.colorAx
+    simp [colorAx] at this
+    specialize this ((maximalFan G C x y h).val.toList.length - 1) (by simp; apply Nat.sub_lt_sub_right hsize hlt)
+    simp at this;
+
+    have aux : (maximalFan G C x y h).val.size - 1 + 1 = (maximalFan G C x y h).val.size := by
+      apply Nat.sub_add_cancel hsize
+    simp_rw [aux] at this
+
+    specialize aux0 ((maximalFan G C x y h).val.toList.length - 1) (Nat.sub_one_lt (Nat.ne_zero_of_lt hsize))
+    simp at aux0
+    rw [← aux0] at this
+    
+
+    have := add_maximal G C x y (default G C x y h).val ((nbhd G x).val.erase y) (default G C x y h).nonemptyAx
+    simp [Array.back] at this
+    specialize this F.val[(maximalFan G C x y h).val.size] (by sorry )
+    simp_all [maximalFan, mkMaxFan]
+  · apply Array.toList_inj.mp
+    apply List.IsPrefix.eq_of_length_le
+    simp_all
+    sorry
+    exact Nat.le_of_eq heq
 
 end Subfan
